dafny/src/utils/Array.dfy
@@ -1,0 +1,45 @@
+module Arrays {
+
+
+  /* For an element that occurs at least once in a sequence, the index of its
+     first occurrence is returned. */
+  function {:opaque} IndexOf<T(==)>(xs: seq<T>, v: T): (i: nat)
+    requires v in xs
+    ensures i < |xs| && xs[i] == v
+    ensures forall j :: 0 <= j < i ==> xs[j] != v
+  {
+    if xs[0] == v then 0 else 1 + IndexOf(xs[1..], v)
+  }
+  
+     /**
+     * Everything is the same, except for those elements within the given region.
+     */
+    predicate EqualsExcept<T(==)>(lhs:seq<T>, rhs:seq<T>, address:nat, length: nat)
+    // Data region must be within available memory
+    requires address + length <= |lhs| {
+        // Memory sizes are the same
+        |lhs| == |rhs| &&
+        // Check nothing below data region changed
+        lhs[..address] == rhs[..address] &&
+        // Check nothing above data region changed
+        lhs[address+length..] == rhs[address+length..]
+    }
+    /**
+     * Copy a sequence of bytes from into another at a given starting position.
+     */
+    opaque function Copy<T>(src: seq<T>, dst: seq<T>, start: nat) : (result:seq<T>)
+    // Must have enough space in the destination sequence.
+    requires (start+|src|) <= |dst|
+    // Resulting array unchanged in size
+    ensures |result| == |dst|
+    // Affected region matches source array
+    ensures src == result[start .. (start+|src|)]
+    // Everything unchanged outside affected region
+    ensures EqualsExcept(dst,result,start,|src|)
+    {
+        // Precompute end within destination
+        var end := start+|src|;
+        // Construct the sequence!
+        seq(|dst|, i requires i >= 0 && i < |dst| => if (i >= start && i<end) then src[i-start] else dst[i])
+    }
+}
